src/Helpers/Varmap.v
@@ -1,0 +1,41 @@
+Require PeanoNat.
+
+Set Implicit Arguments.
+
+Class Default A := default_val: A.
+
+Instance def_f A B {def:Default B} : Default (A -> B) := fun _ => default_val.
+Instance def_pair A B {defA:Default A} {defB:Default B}
+  : Default (A*B) := (default_val, default_val).
+Instance def_type : Default Type := unit.
+
+Hint Extern 1 (Default _) => solve [ constructor ] : typeclass_instances.
+
+Module varmap.
+  Definition I := nat.
+  Inductive t (A:Type) : Type :=
+  | empty
+  | cons (i:I) (x:A) (xs:t A).
+
+  Definition index_eq (i1 i2:I) : bool :=
+    Nat.eqb i1 i2.
+
+  Theorem index_eq_prop : forall i1 i2,
+      index_eq i1 i2 = true <-> i1 = i2.
+  Proof.
+    apply PeanoNat.Nat.eqb_eq.
+  Qed.
+
+  Fixpoint find {A} `{Default A} (i:nat) (vm: t A) : A :=
+    match vm with
+    | empty _ => default_val
+    | cons i' x vm' => if Nat.eqb i i' then x else find i vm'
+    end.
+
+  Fixpoint length A (ctx: t A) : nat :=
+    match ctx with
+    | empty _ => O
+    | cons _ _ ctx' => S (length ctx')
+    end.
+
+End varmap.
